src/Unfolder.v
@@ -15,32 +15,6 @@ Require NatMap.
 Module FM := NatMap.IntMap.
 
 
-Lemma applyD_impl_Forall : forall types F F' P Dom args R D v,
-  applyD (types := types) F Dom args R D = Some v ->
-  Forall P args ->
-  (forall x y v, P x -> F x y = Some v -> F' x y = Some v) ->
-  applyD F' Dom args R D = Some v.
-Proof.
-  induction Dom; destruct args; simpl; intros; think; auto. inversion H0; subst; intros.
-  erewrite H1; eauto.
-Qed.
-
-Lemma applyD_impl : forall types F F' Dom args R D,
-  (forall x y, F x y = F' x y) ->
-  applyD (types := types) F Dom args R D = applyD F' Dom args R D.
-Proof.
-  induction Dom; destruct args; simpl; intros; think; auto.
-  destruct (F' e a); auto.
-Qed.
-
-Lemma applyD_map : forall types F F' Dom args R D,
-  applyD (types := types) F Dom (map F' args) R D = applyD (fun x y => F (F' x) y) Dom args R D.
-Proof.
-  induction Dom; destruct args; simpl; intros; think; auto.
-  destruct (F (F' e) a); auto.
-Qed.
-
-
 Module Make (SH : SepHeap) (U : SynUnifier).
   Module Import SE := SH.SE.
   Import SH.
@@ -111,12 +85,13 @@ Module Make (SH : SepHeap) (U : SynUnifier).
 
     End instantiate.
 
+(*
     Definition applySHeap (F : expr types -> expr types) (sh : SHeap types pcType stateType) : SHeap types pcType stateType :=
       {| impures := MM.mmap_map (map F) (impures sh)
        ; pures := map F (pures sh)
        ; other := other sh
        |}.
-
+*)
 
     (** Preprocessed databases of hints *)
 
@@ -447,9 +422,9 @@ Module Make (SH : SepHeap) (U : SynUnifier).
                    | [ |- match ?X with _ => _ end = match ?X with _ => _ end ] =>
                      consider X; intros; try reflexivity
                  end; think; auto.
-        eapply nth_error_typeof_funcs in H2; eauto. intuition. think.
-        { rewrite applyD_map.
-          revert H1. destruct s; simpl in *. clear H5. generalize dependent Domain. clear - H.
+        { unfold typeof_funcs in H0. rewrite map_nth_error_full in H0. rewrite H3 in H0. inversion H0; clear H0; subst.
+          destruct s; simpl in *; subst; clear - H H2. rewrite applyD_map.
+          revert H2. generalize dependent Domain. clear - H.
           induction H; destruct Domain; intros; simpl in *; think; auto.
           consider (exprD funcs (U ++ F) G (openForUnification (length U) x) t); intros; auto. }
       Qed.
@@ -471,7 +446,7 @@ Module Make (SH : SepHeap) (U : SynUnifier).
                    | [ |- match ?X with _ => _ end = match ?X with _ => _ end ] =>
                      consider X; intros; try reflexivity
                  end; think; auto.
-        { rewrite EquivDec_refl_left. reflexivity. }
+        { rewrite tvar_seqb_refl. reflexivity. }
         { destruct t0; simpl in *. clear H0. generalize dependent TDomain. induction H; destruct TDomain; simpl in *; auto.
           intros; think; auto. }
       Qed.
@@ -512,7 +487,7 @@ Module Make (SH : SepHeap) (U : SynUnifier).
           rewrite <- app_nil_r with (l := G); eauto using exprD_weaken.
           rewrite <- app_nil_r with (l := U); eauto using exprD_weaken. }
         { unfold typeof_funcs in H0; rewrite map_nth_error_full in H0. rewrite H2 in H0. inversion H0; clear H0; subst.
-          unfold typeof_sig in *. simpl in *. destruct s. revert H4 H1. clear - H. generalize dependent Domain.
+          destruct s; simpl in *. revert H5 H1. clear - H. generalize dependent Domain.
           induction H; destruct Domain; simpl in *; intros; think; auto.
           erewrite <- H; eauto. destruct (exprD funcs nil (G' ++ F) x t); auto. }
       Qed.
@@ -578,17 +553,17 @@ Module Make (SH : SepHeap) (U : SynUnifier).
                    | [ |- context [ NPeano.ltb ?X ?Y ] ] => consider (NPeano.ltb X Y); intros
                  end; think); auto.
         { destruct U_or_G; simpl; rewrite nth_error_app_R by omega.
-          cutrewrite (x + length U - length U = x); [ | omega ]. rewrite H. rewrite EquivDec_refl_left; auto.
-          cutrewrite (x + length G - length G = x); [ | omega ]. rewrite H. rewrite EquivDec_refl_left; auto. }
+          cutrewrite (x + length U - length U = x); [ | omega ]. rewrite H. rewrite tvar_seqb_refl; auto.
+          cutrewrite (x + length G - length G = x); [ | omega ]. rewrite H. rewrite tvar_seqb_refl; auto. }
         { consider (U.Subst_lookup (length U + x - length G') sub); intros.
-          generalize H3. eapply U.WellTyped_lookup in H3; eauto. destruct H3. intuition. 
+          generalize H4. eapply U.WellTyped_lookup in H4; eauto. destruct H4. intuition. 
           assert (is_well_typed (typeof_funcs funcs) U G e x0 = true).
           { eapply checkAllInstantiated_dropU. eauto. instantiate (1 := nil). rewrite app_nil_r. auto.
             2: eauto. 2: eauto. omega. }
-          clear H6.
-          rewrite nth_error_app_R in H5 by omega. 
-          cutrewrite (length U + x - length G' - length U = x - length G') in H5; [ | omega ].
-          rewrite H in H5; inversion H5; clear H5; subst. destruct U_or_G; simpl.
+          clear H7.
+          rewrite nth_error_app_R in H6 by omega. 
+          cutrewrite (length U + x - length G' - length U = x - length G') in H6; [ | omega ].
+          rewrite H in H6; inversion H6; clear H6; subst. destruct U_or_G; simpl.
           rewrite <- app_nil_r with (l := G); eapply is_well_typed_weaken; eauto.
           rewrite <- app_nil_r with (l := U); eapply is_well_typed_weaken; eauto.
           
@@ -818,58 +793,7 @@ Module Make (SH : SepHeap) (U : SynUnifier).
         { destruct t; try congruence. eapply IHe; eauto. }
       Qed.
 
-      Lemma applySHeap_spec : forall cs U G U' G' s F,
-        (forall e t, 
-          is_well_typed (typeof_funcs funcs) (typeof_env U) (typeof_env G) e t = true ->
-          exprD funcs U G e t = exprD funcs U' G' (F e) t) ->
-        WellTyped_sheap (typeof_funcs funcs) (typeof_preds preds) (typeof_env U) (typeof_env G) s = true ->
-        SE.ST.heq cs (sexprD funcs preds U G (sheapD s))
-                     (sexprD funcs preds U' G' (sheapD (applySHeap F s))).
-      Proof.
-        clear. intros. rewrite WellTyped_sheap_eq in H0. apply andb_true_iff in H0. destruct H0. 
-        do 2 rewrite SH.sheapD_def. simpl. repeat eapply SE.ST.heq_star_frame.
-        { revert H0. clear H1. rewrite WellTyped_impures_spec_eq. eapply MM.PROPS.map_induction with (m := impures s); intros.
-          repeat rewrite SH.impuresD_Empty by eauto using MF.map_Empty. reflexivity.
-          rewrite SH.impuresD_Add by eauto using MF.map_Add, MF.map_not_In.
-          symmetry. unfold MM.mmap_map in *. rewrite SH.impuresD_Add. 2: eapply MF.map_Add; eauto. 
-          2: eapply MF.map_not_In; eauto.
-          simpl. symmetry. rewrite NatMap.IntMapProperties.fold_Add in H3. 5: eauto. 5: eauto.
-          apply andb_true_iff in H3. destruct H3. apply ST.heq_star_frame.
-          cut (ST.heq cs (sexprD funcs preds U G SE.Emp) (sexprD funcs preds U' G' SE.Emp)); [ | reflexivity ].
-          generalize (@SE.Emp types pcType stateType). revert H. clear - H4.
-          induction e; simpl; intros. repeat rewrite starred_nil. auto.
-          repeat rewrite starred_cons. simpl in *. apply ST.heq_star_frame; eauto. 
-          unfold typeof_preds in H4. rewrite map_nth_error_full in H4.
-          destruct (nth_error preds x); try reflexivity.
-          consider (all2 (is_well_typed (typeof_funcs funcs) (typeof_env U) (typeof_env G)) a (typeof_pred p)). intros.
-          rewrite applyD_map. revert H1. clear -H. destruct p; simpl. generalize dependent SDomain0.
-          { induction a; destruct SDomain0; intros; simpl; auto; try reflexivity.
-            simpl in H1. consider (is_well_typed (typeof_funcs funcs) (typeof_env U) (typeof_env G) a t); intros.
-            rewrite H; eauto. destruct (exprD funcs U' G' (F a) t); eauto. reflexivity. }
-          { destruct (nth_error (typeof_preds preds) x); try congruence.
-            consider (all2 (is_well_typed (typeof_funcs funcs) (typeof_env U) (typeof_env G)) a t); intros.
-            destruct e. simpl; repeat rewrite starred_nil. eauto.
-            generalize dependent (e :: e0); intros.
-            eapply IHe; eauto. }
-          { eapply H0; eauto. }
-          { unfold Basics.flip; constructor; eauto. }
-          { clear. unfold Basics.flip. repeat (red; intros; subst). auto. }
-          { clear. repeat (red; intros; subst). repeat rewrite <- andb_assoc. f_equal. apply andb_comm. } }
-        { cut (ST.heq cs (sexprD funcs preds U G SE.Emp) (sexprD funcs preds U' G' SE.Emp)); [ | reflexivity ].
-          revert H1. clear H0. generalize (@SE.Emp types pcType stateType). induction (pures s); intros; 
-          repeat (rewrite starred_nil || rewrite starred_cons); auto. simpl map. rewrite starred_cons.
-          simpl. simpl in H1.
-          consider (is_well_typed (typeof_funcs funcs) (typeof_env U) (typeof_env G) a tvProp); intros.
-          rewrite IHl; eauto. rewrite H; auto. reflexivity. }
-        { cut (ST.heq cs (sexprD funcs preds U G SE.Emp) (sexprD funcs preds U' G' SE.Emp)); [ | reflexivity ].
-          generalize (@SE.Emp types pcType stateType). induction (other s); intros.
-          etransitivity. rewrite starred_nil. reflexivity. etransitivity; [ | rewrite starred_nil; reflexivity ].
-          auto.
-          
-          etransitivity; [ rewrite starred_cons; reflexivity | ].
-          etransitivity; [ |  rewrite starred_cons; reflexivity ]. simpl. rewrite IHl; eauto. reflexivity. }
-      Qed.
-
+(*
       (** TODO : Move to Expr **)
       Lemma typeof_env_app : forall l r,
         typeof_env (types := types) l ++ typeof_env r = typeof_env (l ++ r).
@@ -882,12 +806,14 @@ Module Make (SH : SepHeap) (U : SynUnifier).
       Proof.
         clear. induction g; simpl; auto. rewrite <- typeof_env_app. simpl. rewrite IHg. auto.
       Qed.
+*)
 
       Lemma quant_nil : forall T ug U, quant (T := T) ug U nil = U.
       Proof.
         clear; destruct ug; simpl; intros; try reflexivity. rewrite app_nil_r; auto.
       Qed.
 
+(*
       Lemma applySHeap_typed : forall U G U' G' s F,
         (forall e t, 
           is_well_typed (typeof_funcs funcs) U G e t = true ->
@@ -906,8 +832,7 @@ Module Make (SH : SepHeap) (U : SynUnifier).
         rewrite all2_map_1. erewrite all2_impl; eauto. congruence.
         rewrite allb_map. eapply allb_impl; eauto.
       Qed.
-
-
+*)
 
       Theorem applicableOk : forall U_or_G U G cs facts lem args args' sub TS,
         lemmaD funcs preds nil nil lem ->
@@ -971,20 +896,20 @@ Module Make (SH : SepHeap) (U : SynUnifier).
             split.
             { etransitivity. etransitivity; [ | eapply H ].
               apply ST_EXT.himp_existsEach; intros.
-
-              rewrite <- applySHeap_spec. reflexivity. intros. eauto. rewrite <- rev_length with (l := G0).
-              eapply liftInstantiate_spec; eauto. rewrite typeof_env_app. auto.
-              cutrewrite (s0 = snd (hash (Lhs lem))). rewrite <- typeof_env_app.
+              
+              erewrite <- applySHeap_wt_spec. reflexivity. intros. eauto. rewrite <- rev_length with (l := G0).
+              eapply liftInstantiate_spec; eauto. rewrite <- typeof_env_app. auto.
+              cutrewrite (s0 = snd (hash (Lhs lem))). rewrite typeof_env_app.
               rewrite typeof_env_rev.
               cutrewrite (typeof_env G0 = fst (hash (Lhs lem))).
               eapply WellTyped_hash. simpl typeof_env. apply Subst_to_env_typeof_env in H11. rewrite <- H11. auto.
               rewrite H10; auto. rewrite H10; auto.
 
               apply ST_EXT.himp_existsEach. intros.
-              rewrite <- applySHeap_spec. reflexivity. intros. rewrite <- rev_length with (l := G0).
-              eapply liftInstantiate_spec; eauto. rewrite typeof_env_app. auto.
+              rewrite <- applySHeap_wt_spec. reflexivity. intros. rewrite <- rev_length with (l := G0).
+              eapply liftInstantiate_spec; eauto. rewrite <- typeof_env_app. auto.
 
-              cutrewrite (s = snd (hash (Rhs lem))). rewrite <- typeof_env_app. rewrite typeof_env_rev. 
+              cutrewrite (s = snd (hash (Rhs lem))). rewrite typeof_env_app. rewrite typeof_env_rev. 
               cutrewrite (typeof_env G0 = v). cutrewrite (v  = fst (hash (Rhs lem))).
               eapply WellTyped_hash. simpl. apply Subst_to_env_typeof_env in H11. rewrite <- H11. auto.
               rewrite H9. auto. subst. reflexivity. rewrite H9. reflexivity. }
@@ -1048,6 +973,7 @@ Module Make (SH : SepHeap) (U : SynUnifier).
         intros. inversion H1; subst; auto.
       Qed.
 
+(*
       Lemma applySHeap_singleton : forall meta_env vars_env cs F f l,
         heq funcs preds meta_env vars_env cs
         (sheapD (applySHeap F
@@ -1066,6 +992,7 @@ Module Make (SH : SepHeap) (U : SynUnifier).
         red; reflexivity. intro; eapply MM.FACTS.empty_in_iff; eassumption.
         red; reflexivity. intro; eapply MM.FACTS.empty_in_iff; eassumption.
       Qed.
+*)
 
       Opaque ST_EXT.existsEach.
 
@@ -1158,8 +1085,8 @@ Module Make (SH : SepHeap) (U : SynUnifier).
           { destruct H6. rewrite H3 in *. rewrite SH.hash_Func in *. rewrite H7 in *.
             rewrite ST_EXT.existsEach_nil in *.
             rewrite SH.hash_denote with (s := Func f x1). rewrite SH.hash_Func.
-            unfold fst, snd, SE.existsEach. subst.
-            rewrite applySHeap_singleton in *. simpl in *. rewrite app_nil_r in *. destruct H11. rewrite H6. clear H6.
+            unfold fst, snd, SE.existsEach. subst. 
+            rewrite HEAP_FACTS.applySHeap_singleton in *. simpl in *. rewrite app_nil_r in *. destruct H11. rewrite H6. clear H6.
             rewrite ST.heq_star_comm. rewrite ST_EXT.heq_pushIn. rewrite rw_skipn_app; eauto with list_length.
             rewrite ST_EXT.existsEach_rev. split. 
             { eapply ST.heq_defn. eapply ST_EXT.heq_existsEach; intros.
@@ -1409,7 +1336,7 @@ Module Make (SH : SepHeap) (U : SynUnifier).
               repeat (rewrite app_nil_r || rewrite app_ass). reflexivity.
               repeat rewrite app_length. rewrite typeof_env_length. subst. rewrite map_length. reflexivity.
               rewrite H4. repeat rewrite app_length. subst. rewrite H1. repeat rewrite map_length.
-              unfold WellTyped_env. rewrite <- typeof_env_app. f_equal.
+              unfold WellTyped_env. rewrite typeof_env_app. f_equal.
               
               repeat match goal with
                        | [ H : _ = _ |- _ ] => rewrite H in *
@@ -1444,7 +1371,7 @@ Module Make (SH : SepHeap) (U : SynUnifier).
             2: rewrite <- typeof_env_length; reflexivity.
             rewrite ST_EXT.existsEach_app. eapply ST_EXT.himp_existsEach. intros.
             eapply IHbound in H4.
-            Focus 2. rewrite H7. instantiate (1 := meta_env ++ G). unfold WellTyped_env. rewrite <- typeof_env_app.
+            Focus 2. rewrite H7. instantiate (1 := meta_env ++ G). unfold WellTyped_env. rewrite typeof_env_app.
             f_equal. symmetry; auto.
             Focus 2. rewrite H5. apply typeof_env_WellTyped_env.
             Focus 2. apply H6. 
